{
 "cells": [
  {
   "cell_type": "markdown",
   "id": "844f803d-f51e-4d3e-946d-94f88875a4e2",
   "metadata": {},
   "source": [
    "$\\textbf{LESSON 1: ASSIGNMENT ANSWERS}$\n",
    "-"
   ]
  },
  {
   "cell_type": "markdown",
   "id": "34ff3e63-2c97-46f8-a83a-17f07bbbd959",
   "metadata": {},
   "source": [
    "$\\textbf{1. Recall the definition of a rational number, denoted as $\\mathbb{Q}$. Prove that the Euler's number $e = \\Sigma_{k=0}^\\infty \\frac{1}{k!} \\notin \\mathbb{Q}$}$\n",
    "$\\textbf{A factorial is defined as $k! = (k)(k-1)(k-2)(k-3)..., \\forall k \\in \\mathbb{Z}^+$, note that $0! = 1$.}$. \n",
    "$\\textbf{Furthermore, a sum notation $\\Sigma_{k=0}^\\infty k = 0+ 1 + 2 + 3 +....+...$}$}$."
   ]
  },
  {
   "cell_type": "markdown",
   "id": "709b75fb-fca2-49ca-b3b7-c17e742c0580",
   "metadata": {},
   "source": [
    "$\\text{Answer:}$\n",
    "\n",
    "Proof by Contradiction:\n",
    "\n",
    "- Suppose, $e = \\frac{m}{n}$\n",
    "\n",
    "Step 1: \n",
    "\n",
    "\\begin{gather}\n",
    "\\frac{m}{n} = \\Sigma_{k=0}^\\infty \\frac{1}{k!} \\\\\n",
    "n! ( \\frac{m}{n} = \\Sigma_{k=0}^\\infty \\frac{1}{k!} ) n!\\\\\n",
    "\\frac{m}{n}n! = \\Sigma_{k=0}^\\infty \\frac{n!}{k!} \\\\\n",
    "m(n-1)! = \n",
    "\\end{gather}\n",
    "\n",
    "Step 2: Expand\n",
    "\n",
    "\\begin{gather}\n",
    "\\Sigma_{k=0}^\\infty \\frac{n!}{k!} =\n",
    "n! + \\frac{n!}{1!} + \\frac{n!}{2!} + ... + \\frac{n!}{n!} + \\frac{n!}{(n + 1)!} + \\frac{n!}{(n + 2)!} + ...\n",
    "\\end{gather}\n",
    "\n",
    "Step 3: Separate finite set and infinite set\n",
    "\n",
    "\\begin{gather}\n",
    "\\Sigma_{k=0}^n \\frac{n!}{k!} = n! + \\frac{n!}{1!} + \\frac{n!}{2!} + ... + \\frac{n!}{n!} \\\\\n",
    "\\Sigma_{k=n + 1}^\\infty \\frac{n!}{k!} = \\frac{n!}{(n + 1)!} + \\frac{n!}{(n + 2)!} + ...\n",
    "\\end{gather}\n",
    "\n",
    "Step 4: \n",
    "\n",
    "\\begin{gather}\n",
    "m(n - 1)! = \\Sigma_{k=0}^n \\frac{n!}{k!} + \\Sigma_{k=n + 1}^\\infty \\frac{n!}{k!}\n",
    "\\end{gather}\n",
    "\n",
    "- We know that $m(n-1)!$, is an integer, therefore, when we add $\\Sigma_{k=0}^n \\frac{n!}{k!}$ and $\\Sigma_{k=n + 1}^\\infty \\frac{n!}{k!}$, they must result into an integer\n",
    "\n",
    "Step 5: Prove $\\Sigma_{k=0}^n \\frac{n!}{k!}$ is an integer\n",
    "\n",
    "\\begin{gather}\n",
    "\\frac{n!}{k!} = \\frac{n(n-1)(n-2)...k(k-1)(k-2)...}{k(k-1)(k-2)...} = n(n-1)(n-2)...\n",
    "\\end{gather}\n",
    "\n",
    "- Therefore, it is an integer\n",
    "\n",
    "Step 6: Contradiction\n",
    "\n",
    "\\begin{gather}\n",
    "\\Sigma_{k=n + 1}^\\infty \\frac{n!}{k!} = \\frac{n!}{(n + 1)!} + \\frac{n!}{(n + 2)!} + \\frac{n!}{(n + 3)!}\\dotsb \\\\ \n",
    "                                      = \\frac{1}{n+1} + \\frac{1}{(n+1)(n+2)} + \\frac{1}{(n+1)(n+2)(n+3)}\\dotsb\\\\\n",
    "                                      = \\frac{1}{n+1} \\begin{bmatrix} 1+\\frac{1}{n+2}+\\frac{1}{(n+2)(n+3)}+\\dotsb \\end{bmatrix}\\\\\n",
    "                                      < \\frac{1}{n+1} \\begin{bmatrix} 1+\\frac{1}{n+1}+\\frac{1}{(n+1)^2}+\\dotsb \\end{bmatrix} \\text{<--Upper Bound which is 1}\n",
    "\\end{gather}\n",
    "\n",
    "Step 7: Continuation\n",
    "\n",
    "- Remember $S = \\frac{a_0}{1 - 3}$ s.t. $a_0 =$ initial value, $r =$ common ratio\n",
    "- Let $a_0 = \\frac{1}{n+1}$, $r = \\frac{1}{n+1}$\n",
    "- Then:\n",
    "\n",
    "\\begin{gather}\n",
    "S = \\frac{\\frac{1}{n+1}}{1 - \\frac{1}{n+1}}\\\\\n",
    "     = \\frac{1}{n} < 1\n",
    "\\end{gather}\n",
    "\n",
    "- Since, the number should be strictly greater than $0$, then:\n",
    "\\begin{gather}\n",
    "0 < \\frac{1}{n} < 1\n",
    "\\end{gather}\n",
    "\n",
    "- There is no Integer between $0$ and $1$, then that contradicts our supposition. Therefore, $e \\notin \\mathbb{Q}$"
   ]
  },
  {
   "cell_type": "markdown",
   "id": "606eeea7-0ebe-409f-b6f7-97e2d2a52a74",
   "metadata": {},
   "source": [
    "$\\textbf{2. Prove Minkowski's Inequality for sums, $\\forall \\ p>1, (a_k, b_k)>0$:}$\n",
    "\\begin{gather} \n",
    "\\begin{bmatrix} \n",
    "\\Sigma_{k=1}^n |a_k + b_k|^p \n",
    "\\end{bmatrix}^\\frac{1}{p}\n",
    "\\leq\n",
    "\\begin{bmatrix} \n",
    "\\Sigma_{k=1}^n |a_k|^p \n",
    "\\end{bmatrix}^ \\frac{1}{p}\n",
    "+\n",
    "\\begin{bmatrix}\n",
    "\\Sigma_{k=1}^n |b_k|^p\n",
    "\\end{bmatrix}^\\frac{1}{p}\n",
    "\\end{gather}"
   ]
  },
  {
   "cell_type": "markdown",
   "id": "f0e14588-7cbe-44e7-8185-59227c63b7ee",
   "metadata": {},
   "source": [
    "$\\text{Answer:}$\n",
    "\n",
    "Step 1: Laws of Exponents (Power raised to a power):\n",
    "\n",
    "- Let $n = $ any base number, then ${(n^p)}^\\frac{1}{p}=n$\n",
    "- Thus,\n",
    "\\begin{gather} \n",
    "\\Sigma_{k=1}^n |a_k + b_k|\n",
    "\\leq\n",
    "\\Sigma_{k=1}^n |a_k|\n",
    "+\n",
    "\\Sigma_{k=1}^n |b_k|\n",
    "\\end{gather}\n",
    "\n",
    "Step 2: Property of Summation (Addition)\n",
    "\n",
    "\\begin{gather} \n",
    "\\Sigma_{k=1}^n |a_k + b_k|\n",
    "\\leq\n",
    "\\Sigma_{k=1}^n |a_k| + |b_k|\n",
    "\\end{gather}\n",
    "\n",
    "Step 3: Prove by Triangle Inequality\n",
    "\n",
    "- Disregarding the Sigma Notation we get:\n",
    "\\begin{gather}\n",
    "|a_k + b_k|\n",
    "\\leq\n",
    "|a_k| + b_k| \n",
    "\\end{gather}\n",
    "\n",
    "- Since, $(a_k, b_k) > 0$, then $(a + b) = a + b$, and $|a| = a_k$, $|b| = b$:\n",
    "- Substitute:\n",
    "\\begin{gather}\n",
    "|a + b| = a + b = |a| + |b|\n",
    "\\end{gather}"
   ]
  },
  {
   "cell_type": "markdown",
   "id": "fd43a720-cf06-441f-8381-98f154cde0c0",
   "metadata": {},
   "source": [
    "$\\textbf{3. Prove the triangle inequality $|x+y| \\leq |x| + |y|, \\forall (x,y) \\in \\mathbb{R}$}$"
   ]
  },
  {
   "cell_type": "markdown",
   "id": "d3107be2-ece1-4b5b-970c-8aa0b8ff31f3",
   "metadata": {},
   "source": [
    "$\\text{Answer:}$\n",
    "\n",
    "Step 1: Definition of an absolute value\n",
    "\n",
    "- Definition\n",
    "\\begin{gather}\n",
    "{|x| = }\n",
    "\\begin{cases}\n",
    "x,&{x \\geq 0}\\\\ -x,&{x < 0}\n",
    "\\end{cases}\n",
    "\\end{gather}\n",
    "\n",
    "- Thus, we must solve for 4 cases:\n",
    "\n",
    "\\begin{gather}\n",
    "\\text{Case 1: }{x \\geq 0, y \\geq 0} \\\\\n",
    "\\text{Case 2: }{x < 0, y < 0} \\\\\n",
    "\\text{Case 3: }{x \\geq 0, y < 0} \\\\\n",
    "\\text{Case 4: }{x < 0, y \\geq 0} \\\\\n",
    "\\end{gather}\n",
    "\n",
    "Case 1: $x \\geq 0, y \\geq 0$\n",
    "\n",
    "- Let, $|x + y| = x + y$, and $|x| = x, |y| = y$\n",
    "- Substitution:\n",
    "\\begin{gather}\n",
    "|x + y| = x + y = |x| + |y|\n",
    "\\end{gather}\n",
    "\n",
    "Case 2: $x < 0, y < 0$\n",
    "\n",
    "- Let, $|x + y| = -(x + y)$, and $|x| = -x, |y| = -y$\n",
    "- Substitution:\n",
    "\\begin{gather}\n",
    "|x + y| = -(x + y) = -x + (-y) = |x| + |y|\n",
    "\\end{gather}\n",
    "\n",
    "Case 3: $x \\geq 0, y < 0$\n",
    "\n",
    "- Let, $|x| = x, |y| = -y$\n",
    "- Substitution:\n",
    "\\begin{gather}\n",
    "|x + y| \\leq x - y\n",
    "\\end{gather}\n",
    "- Since, $x$ and $y$ are different signs, let's consider two sub-cases for $|x + y|$:\n",
    "\\begin{gather}\n",
    "x + y, x + y \\geq 0 \\\\\n",
    "-(x + y), x + y < 0 \\\\\n",
    "\\end{gather}\n",
    "\n",
    "For $x + y \\geq 0$:\n",
    "\\begin{gather}\n",
    "x + y \\leq x - y \\\\\n",
    "y \\leq -y \n",
    "\\end{gather}\n",
    "\n",
    "For $x + y < 0$:\n",
    "\\begin{gather}\n",
    "-(x + y) \\leq x - y \\\\\n",
    "-x - y \\leq x - y \\\\\n",
    "-x \\leq x \n",
    "\\end{gather}\n",
    "\n",
    "Case 4: $x < 0, y \\geq 0$\n",
    "\n",
    "- Let, $|x| = -x, |y| = y$\n",
    "- Substitution:\n",
    "\\begin{gather}\n",
    "|x + y| \\leq -x + y\n",
    "\\end{gather}\n",
    "- Solve for sub-cases of $|x + y|$:\n",
    "\\begin{gather}\n",
    "x + y, x + y \\geq 0 \\\\\n",
    "-(x + y), x + y < 0 \\\\\n",
    "\\end{gather}\n",
    "\n",
    "For $x + y \\geq 0$:\n",
    "\\begin{gather}\n",
    "x + y \\leq -x + y \\\\\n",
    "x \\leq -x\n",
    "\\end{gather}\n",
    "\n",
    "For $x + y < 0$:\n",
    "\\begin{gather}\n",
    "-(x + y) \\leq -x + y \\\\\n",
    "-x - y \\leq -x + y \\\\\n",
    "-y \\leq y\n",
    "\\end{gather}"
   ]
  },
  {
   "cell_type": "markdown",
   "id": "e817c5b4-05d8-4896-a7ca-a1765174f753",
   "metadata": {},
   "source": [
    "$\\textbf{4. Prove Sedrakayan's Lemma $\\forall u_i, v_i \\in \\mathbb{R}^+$:}$\n",
    "\n",
    "\\begin{gather}\n",
    "\\frac{(\\Sigma_{i=1}^n u_i)^2}{\\Sigma_{i=1}^n v_i}\n",
    "\\leq\n",
    "\\Sigma_{i=1}^n \\frac{(u_i)^2}{v_i}\n",
    "\\end{gather}"
   ]
  },
  {
   "cell_type": "markdown",
   "id": "da2bd635-1de2-485c-aeba-cc9bdde55f82",
   "metadata": {},
   "source": [
    "$\\text{Answer:}$\n",
    "\n",
    "Assume $\\frac{a}{b}\\leq c$, then, $a \\leq cb$\n",
    "\n",
    "Therefore:\n",
    "\n",
    "-\n",
    "\\begin{gather}\n",
    "\\frac{(\\Sigma_{i=1}^n u_i)^2}{\\Sigma_{i=1}^n v_i}\n",
    "\\leq\n",
    "\\Sigma_{i=1}^n \\frac{(u_i)^2}{v_i}\n",
    "\\end{gather}\n",
    "-\n",
    "\\begin{gather}\n",
    "(\\Sigma_{i=1}^n u_i)^2\n",
    "\\leq\n",
    "\\Sigma_{i=1}^n \\frac{(u_i)^2}{v_i} (\\Sigma_{i=1}^n v_i)\n",
    "\\end{gather}"
   ]
  },
  {
   "cell_type": "markdown",
   "id": "ee3ffc14-8a17-4632-9934-b55d537884ba",
   "metadata": {},
   "source": [
    "$\\textbf{1. Consider the functions $f(x) = 2x+1$, $g(x)=2y-1$, $j(x) = |f(x)+g(x)|$, and $h(x) = j(x)^2$, show for the following inequality that:}$\n",
    "\n",
    "\\begin{gather}\n",
    "\\sqrt{|f(x)|^2} \\geq \\sqrt{h(x)} - \\sqrt{|g(x)|^2}, \\forall (x,y) \\in \\mathbb{Z}^+\n",
    "\\end{gather}"
   ]
  },
  {
   "cell_type": "markdown",
   "id": "2871d5e0-9c7e-4acd-ac96-063e8c81bfef",
   "metadata": {},
   "source": [
    "$\\text{Answer:}$\n",
    "\n",
    "<b>Step 1:</b> Substitution\n",
    "\n",
    "\\begin{gather}\n",
    "\\sqrt{\\left|f\\left(x\\right)\\right|^2}\\ge \\sqrt{\\left|f\\left(x\\right)+g\\left(x\\right)\\right|^2}-\\sqrt{\\left|g\\left(x\\right)\\right|^2}\n",
    "\\end{gather}\n",
    "\n",
    "<b>Step 2:</b> Minkowski's Inequality for sums\n",
    "\n",
    "\\begin{gather}\n",
    "\\left|f\\left(x\\right)\\right|\\ge \\left|f\\left(x\\right)+g\\left(x\\right)\\right|-\\left|g\\left(x\\right)\\right|\n",
    "\\end{gather}\n",
    "\n",
    "<b>Step 3:</b> Transpose\n",
    "\n",
    "\\begin{gather}\n",
    "\\left|f\\left(x\\right)\\right|+\\left|g\\left(x\\right)\\right|\\ge \\left|f\\left(x\\right)+g\\left(x\\right)\\right|\n",
    "\\end{gather}\n",
    "\n",
    "<b>Step 4:</b> Rearrange to Triangle Inequality\n",
    "\n",
    "\\begin{gather}\n",
    "\\left|f\\left(x\\right)+g\\left(x\\right)\\right|\\le \\left|f\\left(x\\right)\\right|+\\left|g\\left(x\\right)\\right|\n",
    "\\end{gather}\n",
    "\n",
    "<b>Step 5:</b> Prove with the case: $f\\left(x\\right)>0$, and $g\\left(x\\right)>0$, Since $\\forall (x,y) \\in \\mathbb{Z}^+$"
   ]
  },
  {
   "cell_type": "markdown",
   "id": "738b7e70-c75b-4c7d-8e50-2fe9a283404e",
   "metadata": {},
   "source": [
    "Let, $\\left|f\\left(x\\right)+g\\left(x\\right)\\right|=f\\left(x\\right)+g\\left(x\\right)$, and $|x|=x$, $|y|=y$"
   ]
  },
  {
   "cell_type": "markdown",
   "id": "2120248f-2794-4290-8fe1-76cbc7f30137",
   "metadata": {},
   "source": [
    "- Substitute\n",
    "\\begin{gather}\n",
    "\\left|f\\left(x\\right)+g\\left(x\\right)\\right|=f\\left(x\\right)+g\\left(x\\right)=\\left|f\\left(x\\right)\\right|+\\left|g\\left(x\\right)\\right|\n",
    "\\end{gather}"
   ]
  },
  {
   "cell_type": "markdown",
   "id": "183c6f37-f8f9-49aa-a737-27fd42ca0e30",
   "metadata": {},
   "source": [
    "$\\textbf{2. Prove Sedrakayan's Lemma if $u_i, v_i$ are square roots of an even integers:}$\n",
    "\n",
    "\\begin{gather}\n",
    "\\frac{(\\Sigma_{i=1}^n u_i)^2}{\\Sigma_{i=1}^n v_i}\n",
    "\\leq\n",
    "\\Sigma_{i=1}^n \\frac{(u_i)^2}{v_i}\n",
    "\\end{gather}"
   ]
  },
  {
   "cell_type": "markdown",
   "id": "63a90dde-5a4c-48bf-af2c-7b8b595d36c1",
   "metadata": {},
   "source": [
    "To prove Sedrakayan's Lemma when $ u_i $ and $ v_i $ are square roots of even integers:\n",
    "\n",
    "Let $ u_i = \\sqrt{2a_i} $ and $ v_i = \\sqrt{2b_i} $, where $ a_i $ and $ b_i $ are positive integers. We need to show:\n",
    "\n",
    "$$\n",
    "\\frac{\\left( \\sum_{i=1}^n \\sqrt{2a_i} \\right)^2}{\\sum_{i=1}^n \\sqrt{2b_i}} \\leq \\sum_{i=1}^n \\frac{(2a_i)}{(2b_i)}\n",
    "$$\n",
    "\n",
    "Expanding the terms, we get:\n",
    "\n",
    "$$\n",
    "\\frac{\\left( \\sum_{i=1}^n \\sqrt{2a_i} \\right)^2}{\\sum_{i=1}^n \\sqrt{2b_i}} = \\frac{\\left( \\sum_{i=1}^n \\sqrt{2a_i} \\right) \\left( \\sum_{i=1}^n \\sqrt{2a_i} \\right)}{\\sum_{i=1}^n \\sqrt{2b_i}}\n",
    "$$\n",
    "\n",
    "and\n",
    "\n",
    "$$\n",
    "\\sum_{i=1}^n \\frac{(2a_i)}{(2b_i)} = \\sum_{i=1}^n \\frac{2a_i}{2b_i}\n",
    "$$\n",
    "\n",
    "Since $ \\sqrt{2a_i} $ and $ \\sqrt{2b_i} $ are positive, we can rewrite the inequality as:\n",
    "\n",
    "$$\n",
    "\\frac{\\left( \\sum_{i=1}^n \\sqrt{2a_i} \\right)^2}{\\sum_{i=1}^n \\sqrt{2b_i}} \\leq \\sum_{i=1}^n \\frac{\\sqrt{2a_i}^2}{\\sqrt{2b_i}}\n",
    "$$\n",
    "\n",
    "Now, consider the following identity:\n",
    "\n",
    "$$\n",
    "\\left( \\sum_{i=1}^n x_i \\right)^2 = \\sum_{i=1}^n x_i^2 + 2 \\sum_{1 \\leq i < j \\leq n} x_i x_j\n",
    "$$\n",
    "\n",
    "Applying this identity to the numerator, we get:\n",
    "\n",
    "$$\n",
    "\\frac{\\left( \\sum_{i=1}^n \\sqrt{2a_i} \\right)^2}{\\sum_{i=1}^n \\sqrt{2b_i}} = \\frac{\\sum_{i=1}^n (2a_i) + 2 \\sum_{1 \\leq i < j \\leq n} \\sqrt{2a_i} \\sqrt{2a_j}}{\\sum_{i=1}^n \\sqrt{2b_i}}\n",
    "$$\n",
    "\n",
    "Since $2a_i$ and $2b_i$ are even integers, $2 \\sum_{1 \\leq i < j \\leq n} \\sqrt{2a_i} \\sqrt{2a_j}$ is also even.\n",
    "\n",
    "Now, we have:\n",
    "\n",
    "$$\n",
    "\\frac{\\sum_{i=1}^n (2a_i)}{\\sum_{i=1}^n \\sqrt{2b_i}} + \\frac{2 \\sum_{1 \\leq i < j \\leq n} \\sqrt{2a_i} \\sqrt{2a_j}}{\\sum_{i=1}^n \\sqrt{2b_i}} \\leq \\sum_{i=1}^n \\frac{(2a_i)}{\\sqrt{2b_i}}\n",
    "$$\n",
    "\n",
    "Simplifying, we get:\n",
    "\n",
    "$$\n",
    "\\frac{\\sum_{i=1}^n (2a_i)}{\\sum_{i=1}^n \\sqrt{2b_i}} \\leq \\sum_{i=1}^n \\frac{(2a_i)}{\\sqrt{2b_i}}\n",
    "$$\n",
    "\n",
    "Since both sides of the inequality are non-negative, and the numerator of the left-hand side contains the terms of the denominator of the right-hand side, the inequality holds true.\n",
    "\n",
    "Therefore, Sedrakayan's Lemma is proven for $ u_i $ and $ v_i $ being square roots of even integers."
   ]
  }
 ],
 "metadata": {
  "kernelspec": {
   "display_name": "Python 3 (ipykernel)",
   "language": "python",
   "name": "python3"
  },
  "language_info": {
   "codemirror_mode": {
    "name": "ipython",
    "version": 3
   },
   "file_extension": ".py",
   "mimetype": "text/x-python",
   "name": "python",
   "nbconvert_exporter": "python",
   "pygments_lexer": "ipython3",
   "version": "3.11.4"
  }
 },
 "nbformat": 4,
 "nbformat_minor": 5
}
